{
 "cells": [
  {
   "cell_type": "markdown",
   "id": "bf8f8d17-4ed6-4a2e-aac1-4dde9e70d4e4",
   "metadata": {},
   "source": [
    "# Week 8"
   ]
  },
  {
   "cell_type": "markdown",
   "id": "229960ce-0b53-4e92-aea5-569d2ca12969",
   "metadata": {},
   "source": [
    "# Activity 1:\n",
    "\n",
    "### (a)\n",
    "$f(x) = 3x^5 - 10x^2 + 8$\n",
    "\n",
    "Derivative of a polynomial function:\n",
    "\n",
    "$f'(x) = 15x^4 - 20x$\n",
    "\n",
    "### (b)\n",
    "$f(x) = (5x^{12} + 2)(\\pi - \\pi^2 x^4)$\n",
    "\n",
    "Use product rule: $(fg)' = f'g + fg'$\n",
    "\n",
    "$f'(x) = 60x^{11}$\n",
    "\n",
    "$g'(x) = -4\\pi^2 x^3$\n",
    "\n",
    "Apply product rule:\n",
    "\n",
    "$f'(x)g(x) + f(x)g'(x)$\n",
    "\n",
    "$(12\\pi x^{11} - 10\\pi^2 x^{15} - 20\\pi^2 x^3)$\n",
    "\n",
    "### (c)\n",
    "$f(u) = \\sqrt{u} - \\frac{3}{u^3} + 2u^7$\n",
    "\n",
    "Rewrite $\\sqrt{u}$ as $u^{1/2}$ and apply power rule:\n",
    "\n",
    "$f'(u) = \\frac{1}{2} u^{-1/2} + 9u^{-4} + 14u^6$\n",
    "\n",
    "### (d)\n",
    "$f(x) = mx + b \\quad (m, b \\text{ are constants})$\n",
    "\n",
    "Derivative:\n",
    "\n",
    "$f'(x) = m$\n",
    "\n",
    "### (e)\n",
    "$f(x) = 0.5 \\sin{x} + \\frac{\\sqrt[3]{x}}{x} + \\pi^2$\n",
    "\n",
    "Step 1: Derivative of $0.5\\sin{x}$ is $0.5\\cos{x}$\n",
    "\n",
    "Step 2: Rewrite $\\frac{\\sqrt[3]{x}}{x}$ as $x^{-\\frac{2}{3}}$\n",
    "\n",
    "Step 3: Derivative of $x^{-\\frac{2}{3}}$ is $-\\frac{2}{3}x^{-\\frac{5}{3}}$\n",
    "\n",
    "Step 4: The derivative of a constant $\\pi^2$ is 0\n",
    "\n",
    "Final answer:\n",
    "$f'(x) = 0.5\\cos{x} - \\frac{2}{3}x^{-\\frac{5}{3}}$\n",
    "\n",
    "### (f)\n",
    "$f(x) = \\frac{\\pi - \\pi x^4}{5x^{12} + 2}$\n",
    "\n",
    "Use quotient rule: $\\left(\\frac{f}{g}\\right)' = \\frac{f'g - fg'}{g^2}$\n",
    "\n",
    "Let $f(x) = \\pi - \\pi x^4$ and $g(x) = 5x^{12} + 2$\n",
    "\n",
    "Step 1: $f'(x) = -4\\pi x^3$\n",
    "\n",
    "Step 2: $g'(x) = 60x^{11}$\n",
    "\n",
    "Apply quotient rule:\n",
    "\n",
    "$f'(x) = \\frac{(-4\\pi x^3)(5x^{12} + 2) - (\\pi - \\pi x^4)(60x^{11})}{(5x^{12} + 2)^2}$\n",
    "\n",
    "### (g)\n",
    "$f(x) = 2\\sqrt{x} - \\frac{1}{\\sqrt{x}}$\n",
    "\n",
    "Rewrite as: $f(x) = 2x^{1/2} - x^{-1/2}$\n",
    "\n",
    "Step 1: Derivative of $2x^{1/2} is x^{-1/2}$\n",
    "\n",
    "Step 2: Derivative of $-x^{-1/2} is 0.5x^{-3/2}$\n",
    "\n",
    "Final answer:\n",
    "\n",
    "$f'(x) = x^{-1/2} + \\frac{1}{2}x^{-3/2}$\n",
    "\n",
    "### (h)\n",
    "$f(z) = \\tan{z} (\\sin{z} - 5)$\n",
    "\n",
    "Use product rule: $(fg)' = f'g + fg'$\n",
    "\n",
    "Let $f(z) = \\tan{z} and g(z) = \\sin{z} - 5$\n",
    "\n",
    "Step 1: $f'(z) = \\sec^2{z}$\n",
    "\n",
    "Step 2: $g'(z) = \\cos{z}$\n",
    "\n",
    "Apply product rule:\n",
    "\n",
    "$f'(z) = \\sec^2{z}(\\sin{z} - 5) + \\tan{z}\\cos{z}$\n",
    "\n",
    "### (i)\n",
    "$f(x) = \\frac{\\sin{x}}{x^2}$\n",
    "\n",
    "Use quotient rule: $\\left(\\frac{f}{g}\\right)' = \\frac{f'g - fg'}{g^2}$\n",
    "\n",
    "Step 1: $f'(x) = \\cos{x}, g(x) = x^2, g'(x) = 2x$\n",
    "\n",
    "Apply quotient rule:\n",
    "$f'(x) = \\frac{\\cos{x}(x^2) - \\sin{x}(2x)}{x^4}$\n",
    "\n",
    "Final answer:\n",
    "$f'(x) = \\frac{x^2\\cos{x} - 2x\\sin{x}}{x^4}$\n",
    "\n",
    "### (j)\n",
    "$f(x) = x^2 e^x$\n",
    "\n",
    "Use product rule: $(fg)' = f'g + fg'$\n",
    "\n",
    "Step 1: $f'(x) = 2x, g'(x) = e^x$\n",
    "\n",
    "Apply product rule:\n",
    "$f'(x) = 2xe^x + x^2 e^x$\n",
    "\n",
    "### (k)\n",
    "$f(x) = \\cos{x} + e^x$\n",
    "\n",
    "Step 1: Derivative of $\\cos{x} is -\\sin{x}$\n",
    "\n",
    "Step 2: Derivative of $e^x is e^x$\n",
    "\n",
    "Final answer:\n",
    "$f'(x) = -\\sin{x} + e^x$\n",
    "\n",
    "### (l)\n",
    "$f(x) = \\frac{\\sin{x}}{\\cos{x}}$\n",
    "\n",
    "This is the same as $f(x) = \\tan{x}$\n",
    "\n",
    "The derivative of $\\tan{x} is \\sec^2{x}$\n",
    "\n",
    "Final answer:\n",
    "$f'(x) = \\sec^2{x}$\n",
    "\n",
    "### (m)\n",
    "$f(x) = e^x \\ln{\\frac{1}{2x}}$\n",
    "\n",
    "Apply product rule: $(fg)' = f'g + fg'$\n",
    "\n",
    "Let $f(x) = e^x$ and $g(x) = \\ln{\\frac{1}{2x}}$\n",
    "\n",
    "Step 1: $f'(x) = e^x$\n",
    "\n",
    "Step 2: $g'(x) = \\frac{-1}{2x}$\n",
    "\n",
    "Apply product rule:\n",
    "$f'(x) = e^x \\ln{\\frac{1}{2x}} + e^x \\frac{-1}{2x}$\n",
    "\n",
    "### (n)\n",
    "$f(x) = \\frac{10}{10 + \\sin{x}}$\n",
    "\n",
    "Use quotient rule: $\\left(\\frac{f}{g}\\right)' = \\frac{f'g - fg'}{g^2}$\n",
    "\n",
    "Step 1: $f'(x) = 0, g(x) = 10 + \\sin{x}, g'(x) = \\cos{x}$\n",
    "\n",
    "Apply quotient rule:\n",
    "\n",
    "$f'(x) = \\frac{0(10 + \\sin{x}) - 10\\cos{x}}{(10 + \\sin{x})^2}$\n",
    "\n",
    "Final answer:\n",
    "\n",
    "$f'(x) = \\frac{-10\\cos{x}}{(10 + \\sin{x})^2}$\n",
    "\n",
    "### (o)\n",
    "$f(x) = \\sin{(e^x \\cos{x})}$\n",
    "\n",
    "Use chain rule: $f'(x) = \\cos{u} \\cdot u'$\n",
    "\n",
    "Let $u = e^x \\cos{x}$, then $f'(x) = \\cos{(e^x \\cos{x})} \\cdot \\frac{d}{dx} (e^x \\cos{x})$\n",
    "\n",
    "Apply product rule to $u = e^x \\cos{x}$:\n",
    "\n",
    "$u'(x) = e^x \\cos{x} - e^x \\sin{x}$\n",
    "\n",
    "Final answer:\n",
    "\n",
    "$f'(x) = \\cos{(e^x \\cos{x})} \\cdot (e^x \\cos{x} - e^x \\sin{x})$\n",
    "\n",
    "### (p)\n",
    "$f(x) = 6e^{\\cos{t}} / 5\\sqrt[3]{t}$\n",
    "\n",
    "Step 1: Derivative of $6e^{\\cos{t}}$ using chain rule:\n",
    "\n",
    "$\\frac{d}{dt} (6e^{\\cos{t}}) = -6e^{\\cos{t}} \\sin{t}$\n",
    "\n",
    "Step 2: Derivative of $\\frac{1}{5t^{1/3}}$ is $-\\frac{1}{15t^{4/3}}$\n",
    "\n",
    "Final answer:\n",
    "\n",
    "$f'(t) = \\frac{-6e^{\\cos{t}} \\sin{t}}{5\\sqrt[3]{t}} - \\frac{2e^{\\cos{t}}}{15t^{4/3}}$\n",
    "\n",
    "### (q)\n",
    "$f(x) = \\ln{(x^2 + xe^x)}$\n",
    "\n",
    "Use chain rule: $f'(x) = \\frac{1}{u} \\cdot u'$\n",
    "\n",
    "Let $u = x^2 + xe^x$\n",
    "\n",
    "Step 1: Derivative of $u = 2x + e^x + xe^x$\n",
    "\n",
    "Final answer:\n",
    "\n",
    "$f'(x) = \\frac{2x + e^x + xe^x}{x^2 + xe^x}$\n",
    "\n",
    "### (r)\n",
    "$f(x) = \\frac{5x^2 + \\ln{x}}{7\\sqrt{x + 5}}$\n",
    "\n",
    "Use quotient rule: $\\left(\\frac{f}{g}\\right)' = \\frac{f'g - fg'}{g^2}$\n",
    "\n",
    "Step 1: Derivative of $f(x) = 10x + \\frac{1}{x}$\n",
    "\n",
    "Step 2: Derivative of $g(x) = \\frac{7}{2(x+5)^{1/2}}$\n",
    "\n",
    "Apply quotient rule:\n",
    "\n",
    "$f'(x) = \\frac{(10x + \\frac{1}{x})(7\\sqrt{x+5}) - (5x^2 + \\ln{x})\\frac{7}{2(x+5)^{1/2}}}{(7\\sqrt{x+5})^2}$"
   ]
  },
  {
   "cell_type": "markdown",
   "id": "0adf5e2f-f0c5-4a23-ab2c-94401cef431d",
   "metadata": {},
   "source": [
    "# Activity 2\n",
    "\n",
    "### (a)\n",
    "$f(t) + g(t)$\n",
    "\n",
    "Using the sum rule: $(f + g)' = f'(t) + g'(t)$\n",
    "\n",
    "$f'(2) = 2, g'(2) = -1$\n",
    "\n",
    "$f'(2) + g'(2) = 2 + (-1) = 1$\n",
    "\n",
    "### (b)\n",
    "$5f(t) - 2g(t)$\n",
    "\n",
    "Using the constant multiple rule and sum rule:\n",
    "\n",
    "$f'(t) = 2, g'(t) = -1$\n",
    "\n",
    "Derivative: $5f'(t) - 2g'(t)$\n",
    "\n",
    "= $5(2) - 2(-1)$\n",
    "\n",
    "= $10 + 2 = 12$\n",
    "\n",
    "### (c)\n",
    "$f(t)g(t)$\n",
    "\n",
    "Using the product rule: $(fg)' = f'(t)g(t) + f(t)g'(t)$\n",
    "\n",
    "$f'(2) = 2, f(2) = 3, g'(2) = -1, g(2) = 4$\n",
    "\n",
    "$f'(2)g(2) + f(2)g'(2) = 2(4) + 3(-1) = 8 - 3 = 5$\n",
    "\n",
    "### (d)\n",
    "$\\frac{f(t)}{g(t)}$\n",
    "\n",
    "Using the quotient rule: $\\left(\\frac{f}{g}\\right)' = \\frac{f'(t)g(t) - f(t)g'(t)}{g(t)^2}$\n",
    "\n",
    "$f'(2) = 2, f(2) = 3, g'(2) = -1, g(2) = 4$\n",
    "\n",
    "$\\frac{f'(2)g(2) - f(2)g'(2)}{g(2)^2} = \\frac{2(4) - 3(-1)}{4^2} = \\frac{8 + 3}{16} = \\frac{11}{16}$\n",
    "\n",
    "### (e)\n",
    "$g(f(t))$\n",
    "\n",
    "Using the chain rule: $(g(f(t)))' = g'(f(t)) \\cdot f'(t)$\n",
    "\n",
    "$f(2) = 3, f'(2) = 2, g'(3) = 17$\n",
    "\n",
    "$g'(f(2)) \\cdot f'(2) = 17 \\cdot 2 = 34$\n",
    "\n",
    "### (f)\n",
    "$\\sqrt{g(t)}$\n",
    "\n",
    "Using the chain rule: $(\\sqrt{g(t)})' = \\frac{1}{2\\sqrt{g(t)}} \\cdot g'(t)$\n",
    "\n",
    "$g(2) = 4, g'(2) = -1$\n",
    "\n",
    "$\\frac{1}{2\\sqrt{4}} \\cdot (-1) = \\frac{1}{4} \\cdot (-1) = -\\frac{1}{4}$\n",
    "\n",
    "### (g)\n",
    "$t^2 f(t)$\n",
    "\n",
    "Using the product rule: $(t^2 f(t))' = 2t f(t) + t^2 f'(t)$\n",
    "\n",
    "$f(2) = 3, f'(2) = 2$\n",
    "\n",
    "$2(2)(3) + (2^2)(2) = 12 + 8 = 20$\n",
    "\n",
    "### (h)\n",
    "$(f(t))^2 + (g(t))^2$\n",
    "\n",
    "Using the chain rule for both parts: $(f^2)' = 2f(t)f'(t), (g^2)' = 2g(t)g'(t)$\n",
    "\n",
    "$f(2) = 3, f'(2) = 2, g(2) = 4, g'(2) = -1$\n",
    "\n",
    "$2f(2)f'(2) + 2g(2)g'(2) = 2(3)(2) + 2(4)(-1) = 12 - 8 = 4$\n",
    "\n",
    "### (i)\n",
    "$\\frac{1}{f(t)}$\n",
    "\n",
    "Using the chain rule: $\\left(\\frac{1}{f(t)}\\right)' = -\\frac{f'(t)}{f(t)^2}$\n",
    "\n",
    "$f(2) = 3, f'(2) = 2$\n",
    "\n",
    "$-\\frac{f'(2)}{f(2)^2} = -\\frac{2}{3^2} = -\\frac{2}{9}$\n",
    "\n",
    "### (j)\n",
    "$f(3t - (g(1 + t))^2)$\n",
    "\n",
    "Using the chain rule and product rule:\n",
    "\n",
    "Let $u = 3t - (g(1+t))^2$, so $f'(u) = f'(u) \\cdot u'$\n",
    "\n",
    "$u'(t) = 3 - 2g(1+t) \\cdot g'(1+t)$\n",
    "\n",
    "At $t=2: g(1+2) = g(3) = 2, g'(3) = 17$\n",
    "\n",
    "$u'(2) = 3 - 2(2)(17) = 3 - 68 = -65$\n",
    "\n",
    "$f'(u) = f'(2), f'(2) = 2$\n",
    "\n",
    "$f'(u) \\cdot u'(2) = 2 \\cdot (-65) = -130$\n",
    "\n",
    "### (k)\n",
    "To calculate the derivative of $f(g(t))$ at $t = 2$, we would need the value of $g'(2)$ and $f'(g(2))$ to apply the chain rule. We already know $g'(2)$, but we would need $f'(g(2))$.\n",
    "\n",
    "### (l)\n",
    "Estimate the value of $\\frac{f(t)}{g(t)}$ at $t = 1.95$:\n",
    "\n",
    "Using linear approximation: $f(1.95) \\approx f(2) + f'(2)(1.95 - 2) = 3 + 2(-0.05) = 2.9$\n",
    "\n",
    "$g(1.95) \\approx g(2) + g'(2)(1.95 - 2) = 4 + (-1)(-0.05) = 4.05$\n",
    "\n",
    "Estimate: $\\frac{f(1.95)}{g(1.95)} = \\frac{2.9}{4.05} \\approx 0.716$\n"
   ]
  },
  {
   "cell_type": "markdown",
   "id": "1757f242-86ff-466e-bd4a-43d93d079681",
   "metadata": {},
   "source": [
    "# Activity 3: Pseudo Code Derivative Calculator"
   ]
  },
  {
   "cell_type": "code",
   "execution_count": 1,
   "id": "21ba250d-caf4-484a-82eb-2fcf85412b39",
   "metadata": {},
   "outputs": [
    {
     "ename": "SyntaxError",
     "evalue": "invalid syntax (4079608884.py, line 1)",
     "output_type": "error",
     "traceback": [
      "\u001b[0;36m  Cell \u001b[0;32mIn[1], line 1\u001b[0;36m\u001b[0m\n\u001b[0;31m    1. Start\u001b[0m\n\u001b[0m       ^\u001b[0m\n\u001b[0;31mSyntaxError\u001b[0m\u001b[0;31m:\u001b[0m invalid syntax\n"
     ]
    }
   ],
   "source": [
    "1. Start\n",
    "2. Define function `parse_expression(expression)`:\n",
    "   - Tokenize the input algebraic expression.\n",
    "   - Recognize operators (e.g., +, -, *, /) and terms.\n",
    "   - Return a parsed expression in a structured format like a list or tree.\n",
    "\n",
    "3. Define function `differentiate_term(term)`:\n",
    "   - If the term is a constant, return 0.\n",
    "   - If the term is a variable, return 1.\n",
    "   - If the term is a power of a variable, use the power rule:\n",
    "     - Return n * x^(n-1).\n",
    "\n",
    "4. Define function `differentiate_expression(parsed_expression)`:\n",
    "   - For each term in the parsed expression:\n",
    "     - Use `differentiate_term(term)` to compute the derivative of each term.\n",
    "   - Combine the derivatives of each term to form the final derivative expression.\n",
    "   - Return the final derivative expression.\n",
    "\n",
    "5. Define function `simplify_expression(derivative_expression)`:\n",
    "   - Simplify the result such as combining the like terms.\n",
    "   - Return the simplified derivative.\n",
    "\n",
    "6. Define main function `derivative_solver(expression)`:\n",
    "   - Call `parse_expression(expression)` to parse the input expression.\n",
    "   - Call `differentiate_expression(parsed_expression)` to differentiate the parsed expression.\n",
    "   - Call `simplify_expression(derivative_expression)` to simplify the result.\n",
    "   - Output the final derivative.\n",
    "\n",
    "7. End"
   ]
  },
  {
   "cell_type": "code",
   "execution_count": null,
   "id": "1167587b-e441-4af0-90bb-a156b96e1a23",
   "metadata": {},
   "outputs": [],
   "source": []
  }
 ],
 "metadata": {
  "kernelspec": {
   "display_name": "Python 3 (ipykernel)",
   "language": "python",
   "name": "python3"
  },
  "language_info": {
   "codemirror_mode": {
    "name": "ipython",
    "version": 3
   },
   "file_extension": ".py",
   "mimetype": "text/x-python",
   "name": "python",
   "nbconvert_exporter": "python",
   "pygments_lexer": "ipython3",
   "version": "3.10.8"
  }
 },
 "nbformat": 4,
 "nbformat_minor": 5
}
